examples/scalaEquivalenceBenchmarkExamples/ArrayContent.dfy
@@ -1,15 +1,17 @@
 /* Copyright 2009-2024 EPFL, Lausanne */
 
 
-function arrayContentM(a: seq<int>, n: int) : Set[int]
+function arrayContentM(a: seq<int>, n: int) : set<int>
   requires (n >= 0 && n <= |a| && |a| <= 100000)
   decreases(n) {
-  if n == 0  Set.empty[int]
-  else arrayContentM(a, n-1) ++ Set(a(n-1))
+  if n == 0  then {}
+  else arrayContentM(a, n-1) + {a[n-1]}
+  }
 
 
-function arrayContent(a: seq<int>, n: int) : Set[int]
+function arrayContent(a: seq<int>, n: int) : set<int>
   requires (n >= 0 && n <= |a| && |a| <= 100000)
   decreases(n) {
-  if n == 0  Set.empty[int]
-  else Set(a(n-1)) ++ arrayContent(a, n-1)
+  if n == 0  then {}
+  else {a[n-1]} + arrayContent(a, n-1)
+  }
