examples/scalaEquivalenceBenchmarkExamples/MaxHeapify.dfy
@@ -1,57 +1,61 @@
 /* Copyright 2009-2024 EPFL, Lausanne */
 
 
-function maxHeapifyM(a: seq<int>, N: int, i: int): Unit
+function maxHeapifyM(a: seq<int>, N: int, i: int): seq<int>
   requires (i >= 0 && i < N && N <= |a| && N <= 100000)
   decreases(N - i) {
   var l := leftM(i);
   var r := rightM(i);
-  val largest =
-    if l < N && a(l) > a(i) 
+  var largest :=
+    if l < N && a[l] > a[i] then
       l
     else
-      i
-  val largest2 =
-    if r < N && a(r) > a(largest) 
+      i;
+  var largest2 :=
+    if r < N && a[r] > a[largest] then
       r
     else
-      largest
-  if largest2 != i 
-      var temp := a(i);
-      a(i) = a(largest2)
-      a(largest2) = temp
-      maxHeapifyM(a, N, largest2)
+      largest;
+  if (largest2 != i) then
+      var temp := a[i];
+      maxHeapifyM(a[i := a[largest2]][largest2 := temp], N, largest2)
+  else 
+    a
+  }
 
-function leftM(i: int) : int
+function leftM(i: int): int
   requires (0 <= i && i < 100000)
-  2 * i + 1
+  {2 * i + 1}
 
-function rightM(i: int) : int
+function rightM(i: int): int
   requires (0 <= i && i < 100000)
-  2 * i + 2
+  {2 * i + 2}
 
-
-function maxHeapify(a: seq<int>, N: int, i: int): Unit
+function maxHeapify(a: seq<int>, N: int, i: int): seq<int>
   requires (i >= 0 && i < N && N <= |a| && N <= 100000)
   decreases(N - i) {
   var l := 2 * i + 1;
   var r := 2 * i + 2;
-  val largest =
-    if l < N && a(l) > a(i) 
+  var largest :=
+    if l < N && a[l] > a[i] then
       l
     else
-      i
-  val largest2 =
-    if r < N && a(r) > a(largest) 
+      i;
+  var largest2 :=
+    if r < N && a[r] > a[largest] then
       r
     else
-      largest
-  if largest2 != i 
-    swap(i, largest2, a, N)
-    maxHeapify(a, N, largest2)
+      largest;
+  if (largest2 != i) then
+    var newArr := swap(i, largest2, a, N);
+    maxHeapify(newArr, N, largest2)
+  else 
+    a
+  }
 
-function swap(a: int, b: int, array: seq<int>, N: int): Unit
-  requires (a >= 0 && a < N && b >= 0 && b < N && N <= |array| && N <= MAX)
-  var temp := array(a);
-  array(a) = array(b)
-  array(b) = temp
+function swap(a: int, b: int, arr: seq<int>, N: int): seq<int>
+  requires (a >= 0 && a < N && b >= 0 && b < N && N <= |arr| && N <= 100000)
+  {
+    var temp := arr[a];
+    arr[a := arr[b]][b := temp]
+  }
