examples/scalaEquivalenceBenchmarkExamples/fullAlternation.dfy
@@ -15,12 +15,7 @@ function m1(n: int, flag: bool): int {
 function m2(n: int, mode: bool): int {
   if (n < 1) then 0
   else if (n == 1 || n == 2) then 1
-  else {
-    var results: int := 0;
-    if (mode) then
-      {results := m2(n-2, !mode) + m2(n-2, !mode) + m2(n-3, !mode);}
-    else {}
-    if (!mode) then {results := m2(n-1, !mode) + m2(n-2, !mode);} else {}
+  else
+    var results := if (mode) then m2(n-2, !mode) + m2(n-2, !mode) + m2(n-3, !mode) else m2(n-1, !mode) + m2(n-2, !mode);
     results
-  }
 }
