examples/scalaEquivalenceBenchmarkExamples/sum.dfy
@@ -7,9 +7,9 @@
 // Fig. 5 - two functions are not in lock-step
 
 function sum1(n: int): int
-  if (n <= 1) then n
-  else n + n-1 + sum1(n-2)
+  {if (n <= 1) then n
+  else n + n-1 + sum1(n-2)}
 
 function sum2(n: int): int
-  if (n <= 1) then n
-  else n + sum2(n-1)
+  {if (n <= 1) then n
+  else n + sum2(n-1)}
