examples/scalaEquivalenceBenchmarkExamples/unrolling.dfy
@@ -15,7 +15,7 @@ function fact13_1(n: int): int {
 }
 
 function fact13_2(n: int): int
-  if (n <= 1) then 1
+  {if (n <= 1) then 1
   else if (n == 2) then 2
   else if (n == 3) then 6
   else if (n == 4) then 24
@@ -23,4 +23,4 @@ function fact13_2(n: int): int
   else if (n == 6) then 720
   else if (n == 7) then 5040
   else if (n == 8) then 40320
-  else n * (n-1) * (n-2) * (n-3) * fact13_2(n-4)
+  else n * (n-1) * (n-2) * (n-3) * fact13_2(n-4)}
